WIP: Finished proof of current iteration of recv spec

fairneris/examples/no_drop_dup.v
@@ -1,3 +1,4 @@
+From stdpp Require Import list fin_maps.
 From iris.proofmode Require Import proofmode.
 From trillium.program_logic Require Import ectx_lifting.
 From fairneris Require Import model_draft.
@@ -5,11 +6,8 @@ From fairneris.aneris_lang Require Import aneris_lang.
 From fairneris.aneris_lang.state_interp Require Import state_interp state_interp_events.
 From fairneris.aneris_lang.program_logic Require Import aneris_weakestpre.
 
-Definition Aprog shA : expr :=
-  SendTo #(LitSocket shA) #"Hello" #saB.
-
-Definition Bprog shB : expr :=
-  ReceiveFrom #(LitSocket shB).
+Definition Aprog shA : expr := SendTo #(LitSocket shA) #"Hello" #saB.
+Definition Bprog shB : expr := ReceiveFrom #(LitSocket shB).
 
 Section with_Σ.
   Context `{anerisG (fair_model_to_model simple_fair_model) Σ}.
@@ -34,14 +32,16 @@ Section with_Σ.
     iModIntro.
     iIntros (v2' ? ? Hstep).
     pose proof (λ b c d f g h i j k,
-                aneris_events_state_interp_send_untracked {[saA]} b c d f g h _ i _ _ _ _ (inl (ip_of_address saA,tid)) j k Hstep)
+                aneris_events_state_interp_send_untracked {[saA]}
+                  b c d f g h _ i _ _ _ _
+                  (inl (ip_of_address saA,tid)) j k Hstep)
       as Huntracked.
     inv_head_step; iNext.
     rewrite (insert_id (state_sockets σ)); last done.
     rewrite (insert_id (state_sockets σ)) in Huntracked; last done.
     iAssert (socket_address_group_own {[saA]})%I as "#HsaA".
     { iDestruct "Hrt" as "[(%send & %recv & _ & _ & _ & $ & _) _]". }
-        iAssert (socket_address_group_own {[saB]})%I as "#HsaB".
+    iAssert (socket_address_group_own {[saB]})%I as "#HsaB".
     { by iDestruct "Hmsg" as (γ) "[H _]". }
     iMod (aneris_state_interp_send shA saA {[saA]} saB {[saB]} _ _ sA _ _ _ _ _
                                    "Hello"
@@ -82,9 +82,29 @@ Section with_Σ.
     done.
   Admitted.
 
+  Lemma snoc_eq {A} (xs ys : list A) x y :
+    xs ++ [x] = ys ++ [y] → xs = ys ∧ x = y.
+  Proof.
+    revert ys.
+    induction xs.
+    - intros ys Heq. simpl in *.
+      rewrite comm in Heq.
+      apply app_singleton in Heq. set_solver.
+    - intros ys Heq.
+      simpl in *.
+      assert (∃ z zs, ys = z :: zs) as (z & zs & ->).
+      { rewrite app_comm_cons in Heq.
+        destruct ys.
+        { simpl in *. inversion Heq.
+          apply app_nil in H2.
+          set_solver. }
+        set_solver. }
+      set_solver.
+  Qed.
+
   Lemma wp_B shB :
     {{{ shB ↪[ip_of_address saB] sB ∗ saB ⤳ (∅,∅) ∗ saB ⤇ (λ _, True) }}}
-      Bprog shB @[ip_of_address saA]
+      Bprog shB @[ip_of_address saB]
     {{{ v, RET v; True }}}.
   Proof.
     iIntros (Φ) "(Hsh & Hrt & #HΨ) HΦ".
@@ -92,17 +112,121 @@ Section with_Σ.
     iIntros (tid) "Hnode".
     iLöb as "IH".
     iApply wp_lift_head_step; auto.
-    iIntros (ex atr K tp1 tp2 σ Hexvalid Hex) "(Hevs & Hσ & Hm & Hauth) /=".
+    iIntros (ex atr K tp1 tp2 σ Hexvalid Hex) "(Hevs & Hσ & %Hm & Hauth) /=".
     iMod (steps_auth_update_S with "Hauth") as "Hauth".
     rewrite (last_eq_trace_ends_in _ _ Hex).
     iDestruct (aneris_state_interp_socket_valid with "Hσ Hsh")
       as (Sn r) "[%HSn (%Hr & %Hreset)]".
-    iMod (fupd_mask_intro_subseteq _ ∅ True%I with "[]") as "Hmk";
-      first set_solver; auto.
-    iModIntro. iSplitR.
-    { iPureIntro. admit. }
-    iIntros (v2' ? ? Hstep).
-    admit.
+    destruct (decide (r = [])) as [-> | Hneq].
+    - iMod (fupd_mask_intro_subseteq _ ∅ True%I with "[]") as "Hmk";
+        first set_solver; auto.
+      iModIntro. iSplitR.
+      { by iPureIntro; do 3 eexists; eapply SocketStepS; eauto; econstructor. }
+      iIntros (v2' ? ? Hstep).
+      pose proof (λ b c d f g h, aneris_events_state_interp_no_triggered' b c d
+                                 _ f _ _ _ _ (inl (ip_of_address saB,tid)) g h
+                                 Hstep)
+        as Hnotriggered.
+      inv_head_step; [|].
+      + assert (length (r ++ [m]) = length ([] : list message))
+          as Hdone; [by f_equal|].
+        rewrite app_length /= in Hdone. lia.
+      + rewrite (insert_id (state_sockets σ)); last done.
+        rewrite (insert_id (state_sockets σ)) in Hnotriggered; last done.
+        iNext.
+        iMod "Hmk".
+        iModIntro.
+        iExists (trace_last atr), (Some B).
+        rewrite -message_history_evolution_id; iFrame.
+        rewrite Hnotriggered;
+           [|done|done| by intros ? (?&?&?&?&?&?&?&?&?&?&?&?&?) |
+             by intros ? (?&?&?&?&?&?&?&?&?&?&?&?&?) |
+             by intros ? (?&?&?&?&?&?&?&?&?)].
+        iFrame.
+        iSplit.
+        { iPureIntro.
+          rewrite /trace_ends_in in Hex.
+          rewrite /simple_valid_state_evolution.
+          rewrite /simple_valid_state_evolution in Hm.
+          rewrite Hex in Hm=> /=.
+          done. }
+        iApply ("IH" with "[$] [$] [$] [$]").
+    - iClear "IH".
+      iMod (fupd_mask_intro_subseteq _ ∅ True%I with "[]") as "Hmk";
+        first set_solver; auto.
+      iModIntro. iSplitR.
+      { iPureIntro. apply last_is_Some in Hneq as [m Hneq].
+        apply last_Some in Hneq as [? ->].
+        do 3 eexists; eapply SocketStepS; eauto; econstructor; eauto 2. }
+      iIntros (v2' ? ? Hstep).
+      pose proof (λ a b c d f g h i j k,
+                  aneris_events_state_interp_receive_untracked a b c d f g h _ i _ _ _ _ (inl (ip_of_address saB,tid)) j k Hstep)
+        as Huntracked.
+      iAssert (socket_address_group_own {[saB]})%I as "#HsaB".
+      { iDestruct "Hrt" as "[(%send & %recv & _ & _ & _ & $ & _) _]". }
+      inv_head_step.
+      iPoseProof (aneris_state_interp_receive_some saB {[saB]} _ _ _ _ (Some _)
+                      with "[] [$HΨ] [$Hσ] [$Hsh] [Hrt]")
+        as (R' sagT) "(%HinT & #HownT & %Hhist & %HR & Hrt & Hrest)";
+        [by set_solver..| | |].
+      { iFrame "#". iPureIntro. set_solver. }
+      { iDestruct "Hrt" as "[$ Hrt]". }
+      simpl.
+      iClear "Hrt".
+      iNext.
+      iMod "Hmk".
+      iMod "Hrest" as "(Hσ & Hsh & Ha)".
+      iDestruct (Huntracked with "Ha Hevs") as "[Hevs Ha]";
+            [try done..| |].
+      { eexists saB, _, _, _, _, _.
+        repeat split; set_solver. }
+      clear Huntracked.
+      iModIntro.
+      (* TODO: Deduce that we are in [Delivered n m] *)
+      assert (∃ x y, trace_last atr = Received x (S y)) as (x&y&Hatlast).
+      { admit. }
+      iExists (Received x y), (Some B).
+      rewrite Hhist.
+      iFrame.
+      iSplit.
+      { iPureIntro.
+        rewrite /simple_valid_state_evolution. simpl.
+        rewrite /simple_valid_state_evolution in Hm.
+        rewrite Hatlast in Hm. simpl in Hm.
+        rewrite /trace_ends_in in Hex.
+        rewrite Hex in Hm.
+        simpl in Hm.
+        destruct Hm as [Hm1 Hm2].
+        split; [done|].
+        simplify_eq.
+        simpl in *.
+        destruct Hm2 as (shA & shB' & Hm2).
+        rewrite Hm2 in HSn.
+        simpl in *. rewrite insert_commute in HSn; [|done].
+        rewrite lookup_insert in HSn.
+        simplify_eq.
+        assert (shB = shB') as <-.
+        { rewrite lookup_insert_Some in Hr. set_solver. }
+        exists shA, shB.
+        rewrite Hm2.
+        rewrite insert_commute; [|done].
+        rewrite insert_insert.
+        f_equiv.
+        rewrite insert_insert.
+        assert (r0 = mABm y) as ->.
+        { rewrite lookup_insert_Some in Hr.
+          destruct Hr as [[_ Hr]|[Hr _]]; [|done].
+          rewrite /mABm in Hr.
+          replace (S y) with (y + 1)%nat in Hr by lia.
+          rewrite repeat_app in Hr. simpl in Hr.
+          simplify_eq.
+          rewrite /mABm.
+          apply snoc_eq in Hr.
+          set_solver. }
+        done. }
+      iApply wp_value.
+      iExists _. iSplit; [done|].
+      by iApply "HΦ".
   Admitted.
 
 End with_Σ.
